\documentclass{article}
\usepackage[usenames]{color}
\usepackage{minted}
\usepackage[utf8]{inputenc}
\usepackage[T1]{fontenc}
\usepackage{graphicx}
\usepackage{grffile}
% Package longtable omitted
% Package wrapfig omitted
% Package rotating omitted
\usepackage[normalem]{ulem}
\usepackage{amsmath}
\usepackage{textcomp}
\usepackage{amssymb}
% Package capt-of omitted
% Package hyperref omitted
\pagestyle{empty}             % do not remove
% The settings below are copied from fullpage.sty
\setlength{\textwidth}{\paperwidth}
\addtolength{\textwidth}{-3cm}
\setlength{\oddsidemargin}{1.5cm}
\addtolength{\oddsidemargin}{-2.54cm}
\setlength{\evensidemargin}{\oddsidemargin}
\setlength{\textheight}{\paperheight}
\addtolength{\textheight}{-\headheight}
\addtolength{\textheight}{-\headsep}
\addtolength{\textheight}{-\footskip}
\addtolength{\textheight}{-3cm}
\setlength{\topmargin}{1.5cm}
\addtolength{\topmargin}{-2.54cm}

\IfFileExists{./resources/style.sty}{\usepackage{./resources/style}}{}
\IfFileExists{./resources/referencing.sty}{\usepackage{./resources/referencing}}{}
\addbibresource{../Resources/references.bib}
\usepackage[mode=buildnew]{standalone}
\usepackage{tikz}
\usetikzlibrary{decorations.fractals}
\usetikzlibrary{lindenmayersystems}

\begin{document}
$p_{n}=p_{n-1}  \left(\frac{4}{3} \right)$
$s$
\begin{align}
N_{n} &= N_{n-1} \cdot 4 \\
&= 3 \cdot 4^{n}
\end{align}
$l$
$s$
\begin{align}
l = \frac{s \cdot l_{0}}{3^{n}}
\end{align}
\begin{align}
p_{n} &= N_{n} \times l \\
&= 3\cdot 4^{n} \times \frac{s \cdot l_{o}}{3^{n}} \\
&= 3 \cdot s \cdot  l_{0} \left( \frac{4}{3} \right)^{n}
\end{align}
$s$
\begin{align}
s \cdot p_{n} &=  (4/3)^{n} \cdot s \cdot P_{0}\\
& \propto \left(\frac{4}{3}\right)^{n} \\
 \implies  n &= \frac{\ln\left( 4 \right)}{\ln\left( 3 \right)} \label{eq:koch-dim}
\end{align}
$n$
$F$
$\mathbb{R}^n$
$\{U_i: i \in \mathbb{Z}^{+}, U\subset \mathbb{R}^{n}\}$
$\delta$
$U$
$F$
$U$
$\delta$
$F$
\begin{align}
    F \subset \bigcup^\infty_{i=1} \left[ U_i \right] \quad : 0 \leq \left\lvert U_i \right\rvert \leq \delta \label{eq:hausdorff-covering}
\end{align}
$\{U_{i}\}$
$F$
$U_{i}$
$F$
$U_{i}$
$F$
$U_{i}$
$r$
$\frac{r}{2}$
$F$
$\{U_{i}\}$
$\{U_{i}\}$
$\sum^{\infty}_{i=1} \left[\left\lvert U_{i}\right\rvert^{s}\right]$
$U_{i}$
\begin{align}
\mathcal{H}^s_{\delta}\left( F \right)= \inf \left\{ \sum^{\infty}_{i= 1}   \left\lvert U_i \right\rvert^s \enspace : \enspace  \left\{U_i\right\} \text{ is a } \delta \text{-cover of } F \right\}, \quad \delta, s > 0 \label{eq:delta-measure}
\end{align}
$\leq \delta$
$\mathcal{H}^{s}_{\delta} \left(F\right)$
$\delta$
$\matcal{H}_{\delta}^{s}$
$\mathcal{H}^{2}_{\delta}$
$\delta \rightarrow 0$
$s^{th}$
\begin{align}
\mathcal{H}^{s} = \lim_{\delta \rightarrow 0}\left( \mathcal{H}^{s}_{\delta} \right)
\end{align}
$\mathbb{R}^n$
$\mathcal{H}^{2}$
$4\times 1^2 + 4\times \pi\times \frac{1}{2^2} + \frac{1}{2}\times 1 \times \sin{\frac{\pi}{3}}$
$F \subset \mathbb{R^{2}}$
$U_{i}$
$\mathbb{R}^{2}$
$\sqrt{2}$
$\mathcal{H}^{1}$
$\mathcal{H}^{2}$
$\left\lvert U_i \right\rvert^1$
$\left\lvert U_i \right\rvert^2$
$\delta$
$F$
$F$
$s$
\begin{align}
\mathrm{dim}\left(  F \right ) < s \implies \mathcal{H}^{s} \left( F \right)  = \infty
\end{align}
$s$
$F$
$\mathcal{H}^s$
$\infty$
$s$
$s$
\[
\mathcal{H}^s = L \in \mathbb{R}
\]
$t$
$s$
\begin{align*}
0<s<t  \implies   \sum_{i}  \left[ \left\levert U_i \right\rvert^t \right] &= \sum_{i}\left[ \left\levert U_i \right\rvert^{t- s} \cdot  \left\lvert U_i \right\rvert^s \right] \\
&\leq \sum_{i} \left[ \delta^{t - s} \cdot \left\lvert U_i \right\rvert^s  \right]    \\
&= \delta^{t- s}\sum_{i}   \left[ \left\lvert U_i \right\rvert^s \right] 									   \\
\end{align*}
$\lim_{\delta \rightarrow 0}\left[ \sum_{i}   \left\lvert U_i \right\rvert^s \right]$
\begin{align}
    \lim_{\delta \rightarrow 0} \left( \sum_{i}   \left[ \left\lvert U_i \right\rvert^t \right]  \right) & \leq \lim_{\delta}\left( \delta^{t- s} \sum_{i}   \left[ \left\lvert U_i \right\rvert^s \right]  \right) \\
&\leq \lim_{\delta \rightarrow 0}\left( \delta^{t - s} \right) \cdot  \lim_{\delta \rightarrow 0}\left( \sum_{i} \left[ \left\lvert U_i \right\rvert^s \right]    \right) \\
&\leq 0
\end{align}
\begin{align}
    \mathcal{H}^{s} \left(F\right) \in \mathbb{R}  \implies  \mathcal{H}^t\left( F \right)= 0 \quad \forall t > s \label{eq:hdfzero}
\end{align}
$s$
$s = \mathrm{dim}_{H}\left( F \right)$
$F\in \mathbb{R}^{n}$
$\infty$
$F$
$s$
$s$
$\mathcal{H}^{s}$
$\infty$
$\delta$
$\mathbb{R}^{n}$
$0$
$\infty$
$\infty$
\begin{align*}
5 &= 3^D\\
D\ln{3} &= \ln{5}\\
D &= \frac{\ln{5}}{\ln{3}}
\end{align*}
$0^{th}$
$n^{th}$
$k^{th}$
$\binom{n}{k} = \binom{n-1}{k-1} + \binom{n-1}{k}$
$P_{n}$
$2^{n}$
$P_{n+1}$
$P_{n}$
$P_{n+1}$
$n,k \ge 0$
$p$
\begin{equation}
\binom{n}{k} = \prod_{i=0}^{m} \binom{n_i}{k_i} \quad (\text{mod}~p)
\end{equation}
\begin{align*}
n &= n_{m}p^{m}+n_{m-1}p^{m-1}+\cdots + n_{1}p+n_{0},\\
k &= k_{m}p^{m}+k_{m-1}p^{m-1}+\cdots + k_{1}p+k_{0}\\
\end{align*}
$p$
$0$
$1$
$\binom{n}{k} = 0$
$k < n$
$r$
$c$
$P_{n}$
$2^{n}$
$r$
$P_{n+1}$
$2^{n}$
$P_{n}$
$2^{n}$
$c$
$P_{n+1}$
\begin{align*}
\text{Top Triangle:} \quad &\binom{r}{c} \label{eq:top} \\
\text{Bottom-left Triangle:}\quad &\binom{r + 2^n}{c} \label{eq:bottom-left} \\
\text{Bottom-right Triangle :}\quad &\binom{r + 2^n}{c + 2^n} \label{eq:bottom-right}
\end{align*}
$r$
$c$
\begin{align*}
r=r_{i}2^{i}+r_{i-1}2^{i-1}+\cdots + r_{1}2+r_{0}= \left[r_{i}r_{i-1}\cdots r_{1}r_{0}\right]_2\\
c=c_{i}2^{i}+c_{i-1}2^{i-1}+\cdots +c_{1}2+c_{0}=\left[c_{i}c_{i-1}\cdots c_{1}c_{0}\right]_2\\
\end{align*}
\begin{align*}
\binom{2^n + r}{c}~(\text{mod}~2) &= \binom{1r_{i-1}r_{i-2} \cdots r_{0}}{0c_{i-1}c_{i-2} \cdots c_{0}} \quad (\text{mod} 2)\\
&= \binom{1}{0}\binom{r_{i-1}}{c_{i-1}}\binom{r_{i-2}}{c_{i-2}} \cdots \binom{r_0}{c_0} \quad (\text{mod} 2)\\
&=\binom{r_{i-1}}{c_{i-1}}\binom{r_{i-2}}{c_{i-2}} \cdots \binom{r_0}{c_0} \quad (\text{mod} 2)\\
&= \binom{r}{c} \quad (\text{mod} 2)
\end{align*}
\begin{align*}
\binom{2^n + r}{2^n + c}~(\text{mod}~2) &= \binom{1r_{i-1}r_{i-2} \cdots r_{0}}{1c_{i-1}c_{i-2} \cdots c_{0}} \quad (\text{mod} 2)\\
&= \binom{1}{1}\binom{r_{i-1}}{c_{i-1}}\binom{r_{i-2}}{c_{i-2}} \cdots \binom{r_0}{c_0} \quad (\text{mod} 2)\\
&=\binom{r_{i-1}}{c_{i-1}}\binom{r_{i-2}}{c_{i-2}} \cdots \binom{r_0}{c_0} \quad (\text{mod} 2)\\
&= \binom{r}{c} \quad (\text{mod} 2)
\end{align*}
$\binom{r}{c} = \binom{2^n + r}{c} = \binom{2^n + r}{2^n + c} \quad (\text{mod} 2)$
$z \rightarrow z^{2} + \alpha + i
\beta$
$z \rightarrow z^{2} + \alpha + i \beta$
$\varphi$
\[
\mathrm{dim} (\mathtt{my\_fractal}) = \log_{\varphi}=\frac{\log \varphi}{\log 2}
\]
$$\begin{aligned}
G_n &= \frac{F_{n} }{F_{n - 1} } \\
\end{aligned}$$
$$\begin{aligned}
F_n = F_{n- 1} +  F_{n- 2} ; \quad F_1 = F_2 = 1
\end{aligned}$$
$$\begin{aligned}
F_{n} &> 0 \\
0 &< F_{n} \\
 \implies   0 &< F_{n - 2} +  F_{n- 1} \quad \forall n > 2 \\
  F_{n- 2} &< F_{n- 1}  \\
   \implies  F_n & < F_{n+1}
\end{aligned}$$
$$\begin{aligned}
F_{n} &> 0 \\
0 &< F_{n} \\
 \implies   0 &< F_{n - 2} +  F_{n- 1} \quad \forall n > 2 \\
  F_{n- 2} &< F_{n- 1}  \\
   \implies  F_n & < F_{n+1}
\end{aligned}$$
$$\begin{aligned}
G &= \frac{F_{n} +  F_{n+  1} }{F_{n+  1} } \\
&= 1 +  \frac{F_{n- 1} }{F_n} \\
\text{Recall that $F_n > 0 \forall n$}\\
&=  1 +  \frac{1}{    \left\lvert G \right\rvert } \\
 \implies  0 &= G^2- G +  1; \quad G > 0  \\
  \implies  G = \varphi &=  \frac{\sqrt{5} - 1  }{2} \quad  \square
\end{aligned}$$
\[\begin{aligned}
F_{n+ 1} - F_{n} = F_{n- 1} \quad \forall n > 1
\end{aligned}\]
$e^x$
$$\begin{aligned}
\frac{\mathrm{d} }{\mathrm{d} x}\left( e^x \right) \ldots
\end{aligned}$$
$$\begin{aligned}
\lim_{n     \rightarrow \infty }\left[ \frac{F_n}{F_{n- 1} }  \right] &= \varphi \\
\lim_{n     \rightarrow \infty }\left[ \frac{F_n}{F_{n- 1} }  \right] &= \psi \\
\varphi - \psi &=  1 \\
\varphi \times  \psi  &= 1 \\
\frac{\psi}{\varphi}  = \frac{1}{\varphi^2} = \frac{1}{1-\varphi} &= \frac{1}{2-\varphi} = \frac{2}{3 - \sqrt{5}  }
\end{aligned}$$
$\tan^{-1}\left( \frac{1}{1-\varphi}\right)$
$2 \pi \left( \frac{1}{1-\varphi}\right)$
$\log_{\varphi}(2)$
\begin{align}
F_n = F_{n-1} + F_{n-2} \label{eq:fib-def}
\end{align}
$F_{10^{6}}$
\begin{align}
    a_{n}&= a_{n - 1} + a_{n - 2} \nonumber \\
\iff a_{n+  2} &= a_{n+  1} +  a_n \label{eq:fib-def-shift}
\end{align}
\begin{align*}
f''\left( x \right)- f'\left( x \right)- f\left( x \right)=  0
\end{align*}
$y \propto e^{m_{i}x}, \enspace i = 1, 2$
\begin{align*}
f\left( x \right)= e^{mx} = \sum^{\infty}_{n= 0}   \left[ r^{m} \frac{x^n}{n!} \right]
\end{align*}
\begin{align}
    f\left( x \right) &=  \sum^{\infty}_{n= 0}   \left[ a_{n} \cdot  \frac{x^n}{n!} \right]   \label{eq:exp-gen-def-1} \\
 \implies   f'\left( x \right) &=  \sum^{\infty}_{n= 0}   \left[ a_{n+1} \cdot  \frac{x^n}{n!} \right]   \label{eq:exp-gen-def-2} \\
\implies    f''\left( x \right) &=  \sum^{\infty}_{n= 0}   \left[ a_{n+2} \cdot  \frac{x^n}{n!} \right]   \label{eq:exp-gen-def-3}
\end{align}
\begin{align*}
a_{n+  2}    &= a_{n+  1} +  a_{n}\\
\frac{x^n}{n!}   a_{n+  2}    &= \frac{x^n}{n!}\left( a_{n+  1} +  a_{n}  \right)\\
\sum^{\infty}_{n= 0} \left[ \frac{x^n}{n!}   a_{n+  2} \right]        &= \sum^{\infty}_{n= 0}   \left[ \frac{x^n}{n!} a_{n+  1} \right]  + \sum^{\infty}_{n= 0}   \left[ \frac{x^n}{n!} a_{n}  \right]  \\
\end{align*}
\begin{align}
f''\left( x \right) &= f'\left( x \right)+  f\left( x \right)
\end{align}
\begin{align*}
f\left( x \right)= c_1 \cdot  \mathrm{exp}\left[ \left( \frac{1- \sqrt{5} }{2} \right)x \right] +  c_2 \cdot  \mathrm{exp}\left[ \left( \frac{1 +  \sqrt{5} }{2} \right) \right]
\end{align*}
\begin{align*}
f\left( x \right)&= \sum^{\infty}_{n= 0}   \left[ \left( c_1\left( \frac{1- \sqrt{5} }{2} \right)^n +  c_2 \cdot  \left( \frac{1+ \sqrt{5} }{2} \right)^n \right) \cdot  \frac{x^n}{n} \right]
\end{align*}
\begin{align*}
f\left( x \right)= \sum^{\infty}_{n= 0}   \left[ a_n \frac{x^n}{n!} \right]
\end{align*}
\begin{align*}
a_n = c_1\cdot  \left( \frac{1- \sqrt{5} }{2} \right)^n +  c_2 \cdot  \left( \frac{1+  \sqrt{5} }{2} \right)
\end{align*}
\begin{align*}
a_0= c_1 +  c_2  \implies  c_1= - c_2\\
a_1= c_1 \left( \frac{1+ \sqrt{5} }{2} \right) -  c_1 \frac{1-\sqrt{5} }{2}  \implies  c_1 = \frac{1}{\sqrt{5} }
\end{align*}
\begin{align}
    a_n &= \frac{1}{\sqrt{5} } \left[ \left( \frac{1+  \sqrt{5} }{2}  \right)^n -  \left( \frac{1- \sqrt{5} }{2} \right)^n \right] \nonumber \\
&= \frac{\varphi^n - \psi^n}{\sqrt{5} } \nonumber\\
&=\frac{\varphi^n -  \psi^n}{\varphi - \psi} \label{eq:fib-sol}
\end{align}
$\varphi = \frac{1+ \sqrt{5} }{2} \approx 1.61\ldots$
$\psi = 1-\varphi = \frac{1- \sqrt{5} }{2} \approx 0.61\ldots$
\begin{align}
    f\left( x \right) &= \sum^{\infty}_{n= 0}   \left[ a_n \frac{x^n}{n!} \right] \label{eq:exp-pow-series} \\
f'\left( x \right)) &= \frac{\mathrm{d} }{\mathrm{d} x}\left( \sum^{\infty}_{n= 0}   \left[ a_n \frac{x^n}{n!} \right]  \right) \nonumber \\
&= \frac{\mathrm{d}}{\mathrm{d} x} \left( a_0 \frac{x^0}{0!} +  a_1 \frac{x^1}{1!} +  a_2 \frac{x^2}{2!}+  a_3 \frac{x^3}{3! } +  \ldots \frac{x^k}{k!} \right) \nonumber \\
&= \sum^{\infty}_{n= 0}   \left[ \frac{\mathrm{d} }{\mathrm{d} x}\left( a_n \frac{x^n}{n!} \right) \right] \nonumber \\
&= \sum^{\infty}_{n= 0}   {\left[{ \frac{a_n}{{\left({ n- 1 }\right)!}} } x^{n- 1}  \right]} \nonumber \\
\implies f'(x) &= \sum^{\infty}_{n= 0}   {\left[{ \frac{x^n}{n!}a_{n+  1} }\right]} \label{eq:exp-pow-series-sol}
\end{align}
\begin{align}
f^{(k)}\left(x\right) = \sum_{n=0}^\infty\frac{a_{n+k}\cdot x^n}{n!} \quad \text{for}~k \ge 0
\end{align}
$f^{(k)}\left(x\right) = \sum_{n=0}^\infty\frac{a_{n+k}\cdot x^n}{n!}$
$k+1$
$f^{(k+1)}(x) = \sum_{n=0}^\infty\frac{a_{n+k+1}\cdot x^n}{n!}$
\begin{align*}
    \text{LHS} &= f^{(k+1)}(x)\\
    &= \frac{\mathrm{d}}{\mathrm{d}x}\left(f^{(k)}(x)\right)\\
    &= \frac{\mathrm{d}}{\mathrm{d}x}\left(\sum_{n=0}^\infty\frac{a_{n+k}\cdot x^n}{n!}\right)\quad \text{by assumption}\\
    &= \sum_{n=0}^\infty\frac{a_{n+k}\cdot n\cdot x^{n-1}}{n!}\\
    &= \sum_{n=1}^\infty\frac{a_{n+k}\cdot x^{n-1}}{(n-1)!}\\
    &= \sum_{n=0}^\infty\frac{a_{n+k+1}\cdot x^{n}}{n!}\\
    &= \text{RHS}
\end{align*}
\begin{align}
\sum^{n}_{i=0} \left[ c_{i} \cdot f^{(i)}(x) \right] = 0 \label{eq:hom-ode}
\end{align}
$f(x)$
$\frac{\partial }{\partial x}{\left({ f{\left({ x }\right)} }\right)}$
$k$
$k^{\mathrm{th}}$
$k$
$f(x)=c_{i} \cdot e^{m_{i}x}$
$f(x)=c_{i} \cdot x^{j}\cdot e^{m_{i}x}$
$\sum^{k}_{i=0}\left[  c_{i}m^{k-i} \right] = 0$
$\exists i,j \in \mathbb{Z}^{+} \cap \left[0,k\right]$
\begin{align}
\sum^{n}_{i= 0}   \left[ c_i \cdot  a_i \right] = 0, \quad \exists c \in
\mathbb{R}, \enspace \forall i<k\in\mathbb{Z}^+ \nonumber \label{eq:recurrence-relation-def}
\end{align}
\begin{align}
    \sum^{\infty}_{n= 0}   \left[ \sum^{k}_{i= 0}   \left[ \frac{x^n}{n!} c_i a_n \right]  \right]  &= 0 \\
    \sum^{\infty}_{n= 0}    \sum^{k}_{i= 0}    \frac{x^n}{n!} c_i a_n    &= 0 \\
        \sum^{k}_{i= 0} c_i \sum^{\infty}_{n= 0}    \frac{x^n}{n!}  a_n    &= 0
\end{align}
\begin{align}
   \sum^{k}_{i= 0}   \left[ c_i f^{\left( i \right)}\left( x \right) \right]
\end{align}
$f{\left({ x }\right)} \propto e^{m_i x}: \quad m_i \neq m_j \forall i\neq j$
\begin{align}
    f{\left({ x }\right)} = \sum^{k}_{i= 0}   {\left[{ k_i e^{m_i x} }\right]}, \quad \exists m,k \in \mathbb{C} \nonumber
\end{align}
$f{\left({ x }\right)}$
$a_n$
\begin{align}
    \sum^{k}_{i= 0}   {\left[{ k_i e^{m_i x}  }\right]}  &= \sum^{k}_{i= 0}   {\left[{ k_i \sum^{\infty}_{n= 0}   \frac{{\left({ m_i x }\right)}^n}{n!}  }\right]}  \nonumber \\
							 &= \sum^{k}_{i= 0}  \sum^{\infty}_{n= 0}   k_i m_i^n \frac{x^n}{n!} \nonumber\\
							 &=    \sum^{\infty}_{n= 0} \sum^{k}_{i= 0}   k_i m_i^n \frac{x^n}{n!} \nonumber \\
							 &= \sum^{\infty}_{n= 0} {\left[{ \frac{x^n}{n!}  \sum^{k}_{i=0}   {\left[{ k_im^n_i }\right]}  }\right]}, \quad \exists k_i \in \mathbb{C}, \enspace \forall i \in \mathbb{Z}^+\cap {\left[{ 1, k }\right]}     \label{eq:unique-root-sol-power-series-form}
\end{align}
\begin{align}
    f{\left({ x }\right)} &= \sum^{\infty}_{n= 0}   {\left[{  \frac{x^n}{n!} a_n }\right]} \nonumber \\
&= \sum^{\infty}_{n= 0} {\left[{ \frac{x^n}{n!}  \sum^{k}_{i=0}   {\left[{ k_im^n_i }\right]}  }\right]}  \nonumber \\
      \implies  a_n &= \sum^{k}_{n= 0} {\left[{ k_im_i^n }\right]}     \nonumber \\ \nonumber
\square
\end{align}
$m_1 = \varphi, m_2 = {\left({ 1-\varphi }\right)}$
\begin{alignat}{4}
    f{\left({ x }\right)} &= &c_1 e^{\varphi x} +  &c_2 e^{{\left({ 1-\varphi }\right)} x}, \quad &\exists c_1, c_2 \in \mathbb{R} \subset \mathbb{C} \nonumber \\
    \iff  a_n &= &k_1 n^{\varphi} +  &k_2 n^{1- \varphi}, &\exists k_1, k_2 \in \mathbb{R} \subset \mathbb{C} \nonumber
\end{alignat}
\begin{align}
    a_n -  10a_{n+ 1} +  25a_{n+  2}&= 0 \label{eq:hom-repeated-roots-recurrence} \\
    \implies  \sum^{\infty}_{n= 0}   {\left[{ a_n \frac{x^n}{n!} }\right]} - 10 \sum^{\infty}_{n= 0}   {\left[{ \frac{x^n}{n!}+    }\right]} + 25 \sum^{\infty}_{n= 0 }   {\left[{  a_{n+  2 }\frac{x^n}{n!} }\right]}&= 0 \nonumber
\end{align}
\begin{align}
    f''{\left({ x }\right)}- 10f'{\left({ x }\right)}+  25f{\left({ x }\right)}= 0 \nonumber \label{eq:rep-roots-func-ode}
\end{align}
\begin{align}
    m^2- 10m+  25 = 0 \nonumber \\
    {\left({ m- 5 }\right)}^2 = 0 \nonumber \\
    m= 5 \label{eq:rep-roots-recurrence-char-sol}
\end{align}
\begin{align}
    f{\left({ x }\right)}= c_1e^{5x} +  c_2 x e^{5x} \label{eq:rep-roots-ode-sol}
\end{align}
\begin{align}
    x^ke^x &= \sum^{\infty}_{n= 0}   {\left[{ \frac{x^n}{{\left({ n- k }\right)}!} }\right]}, \quad \exists k \in \mathbb{Z}^+ \label{eq:uniq-roots-pow-series-ident}
\end{align}
\begin{align}
    \implies  f{\left({ x }\right)} &= \sum^{\infty}_{n= 0}   {\left[{ c_1 \frac{{\left({ 5x }\right)}^n}{n!} }\right]}  +  \sum^{\infty}_{n= 0}   {\left[{ c_2 n \frac{{\left({ 5x^n }\right)}}{n{\left({ n-1 }\right)}!} }\right]} \nonumber \\
 &= \sum^{\infty}_{n= 0}   {\left[{ \frac{x^n}{n!} {\left({ c_{1}5^n +  c_2 n 5^n   }\right)} }\right]} \nonumber
\end{align}
\begin{align}
    f{\left({ x }\right)}&=     \sum^{\infty}_{n= 0}   {\left[{ a_n \frac{x^n}{n!} }\right]} \nonumber \\
    \iff a_n &= c_{15}^n +  c_2n_5^n \nonumber \\ \nonumber
    \ \nonumber \\
    \square \nonumber
\end{align}
$k^{\mathrm{th}}$
$k$
\begin{align}
     \sum^{k}_{n= 0}   {\left[{ c_i a_n }\right]}  = 0 \nonumber \\
      \implies  \sum^{\infty}_{n= 0}   \sum^{k}_{i= 0}   c_i a_n \frac{x^n}{n!} = 0 \nonumber \\
      \sum^{k}_{i= 0}   \sum^{\infty}_{n= 0}   c_i a_n \frac{x^n}{n!} \nonumber
\end{align}
\begin{align}
    \sum^{k}_{i= 0}   {\left[{ c_if^{{\left({ k }\right)}}  {\left({ x }\right)}    }\right]} \label{eq:gen-form-rep-roots-ode}
\end{align}
$k$
\begin{align}
			 & \sum^{k}_{i= 0}   {\left[{ c_i m^i }\right]} = 0 \wedge m=B, \enspace  \exists! B \in \mathbb{C} \nonumber \\
 \implies      f{\left({ x }\right)}&= \sum^{k}_{i= 0}   {\left[{ x^i A_i e^{mx} }\right]}, \quad \exists A \in \mathbb{C}^+, \enspace \forall i \in {\left[{ 1,k }\right]} \cap \mathbb{N}  \label{eq:sol-rep-roots-ode} \\
\end{align}
\begin{align}
k \in \mathbb{Z} \implies x^k e^x = \sum^{\infty}_{n= 0} {\left[{ \frac{x^n}{{\left({ n- k }\right)}!} }\right]}     \label{eq:power-series-comb}
\end{align}
\begin{align}
f{\left({ x }\right)}&=     \sum^{k}_{i= 0}   {\left[{ A_i \sum^{\infty}_{n= 0}   {\left[{ \frac{{\left({ x m }\right)}^n}{{\left({ n- i }\right)}!} }\right]}  }\right]} \nonumber \\
&=     \sum^{\infty}_{n= 0}   {\left[{ \sum^{k}_{i=0} {\left[{ \frac{x^n}{n!}  \frac{n!}{{\left({ n- i }\right)}} A_i m^n }\right]}       }\right]} # \\
&=     \sum^{\infty}_{n= 0} {\left[{ \frac{x^n}{n!}   \sum^{k}_{i=0} {\left[{  \frac{n!}{{\left({ n- i }\right)}} A_i m^n }\right]}       }\right]}
\end{align}
\begin{align}
f{\left({ x }\right)}&= \sum^{\infty}_{n= 0}   {\left[{ a_n \frac{x^n}{n!} }\right]}      \nonumber \\
 \implies  a_n &= \sum^{k}_{i= 0}   {\left[{ A_i \frac{n!}{{\left({ n- i }\right)}!} m^n  }\right]} \nonumber \\
 &= \sum^{k}_{i= 0}   {\left[{ m^n A_i \prod_{0}^{k} {\left[{ n- {\left({ i- 1 }\right)} }\right]}   }\right]}
& \intertext{$\because \enspace i \leq k$} \notag \\
 &= \sum^{k}_{i= 0} {\left[{ A_i^* m^n n^i }\right]}, \quad \exists A_i \in \mathbb{C}, \enspace \forall i\leqk \in \mathbb{Z}^+ \nonumber \\
\ \nonumber \\
\square \nonumber
\end{align}
$f(x) = xe^x$
\begin{align*}
    xe^x &= 0+\frac{1}{1!}x+\frac{2}{2!}x^2+\frac{3}{3!}x^3+\frac{4}{4!}x^4+\frac{5}{5!}x^5+\dots\\
    &= \sum_{n=0}^\infty \frac{nx^n}{n!}\\
    &= \sum_{n=1}^\infty \frac{x^n}{(n-1)!}
\end{align*}
$f(x) = x^2e^x$
\begin{align*}
    x^2e^x &= \frac{0}{0!} + \frac{0x}{1!} + \frac{2x^2}{2!} + \frac{6x^3}{3!} + \frac{12x^4}{4!} + \frac{20x^5}{5!} + \dots\\
    &= \frac{2\cdot 1x^2}{2!} + \frac{3\cdot 2 x^3}{3!} + \frac{4\cdot 3x^4}{4!} + \frac{5\cdot 4 x^5}{5!} + \dots\\
    &= \sum_{n=2}^\infty \frac{n(n-1)x^n}{n!}\\
    &= \sum_{n=2}^\infty \frac{x^n}{(n-2)!}
\end{align*}
\begin{align*}
    x^ke^x = \sum_{n=k}^\infty \frac{x^n}{(n-k)!} \quad \text{for}~k\in \mathbb{Z^{+}}\cap0
\end{align*}
\begin{align*}
    F_n &= \frac{\varphi^n-\psi^n}{\varphi-\psi} = \frac{\varphi^n-\psi^n}{\sqrt 5} \\
    \iff \frac{F_{n+1}}{F_n}	&= \frac{\varphi^{n+ 1} - \psi^{n+  1}}{\varphi^{n} - \psi^{n}} \\
    \iff \lim_{n \rightarrow \infty}\left[ \frac{F_{n+1}}{F_n} \right]	&= \lim_{n \rightarrow \infty}\left[ \frac{\varphi^{n+ 1} - \psi^{n+  1}}{\varphi^{n} - \psi^{n}} \right] \\
&= \frac{\varphi^{n+ 1} -\lim_{n \rightarrow \infty}\left[ \psi^{n +  1} \right] }{\varphi^{n} - \lim_{n \rightarrow \infty}\left[ \psi^n \right] } \\
\text{because $\mid \psi \mid < 0$ $n \rightarrow \infty \implies \psi^{n} \rightarrow 0$:} \\
&= \frac{\varphi^{n+  1} -  0}{\varphi^{n} -  0} \\
&= \varphi
\end{align*}
$\mathtt{\theta}$
$\pi \mod 1 \approx \frac{1}{7}=0.7142857142857143$
$e \mod 1 \approx \frac{5}{7}= 0.14285714285714285$
$\phi$
$\psi$
$\phi \mod 1 =
\psi$
$\frac{1}{\pi}$
$\theta =2 \varphi  \pi$
$x \rightarrow x^{2}, \enspace x \in \mathbb{R}$
$x>1$
$x<1$
$z \rightarrow z^{2}, \enspace z \in \mathbb{C}$
$\left\lvert z \right\rvert >1$
$\left\lvert z \right\rvert <1$
$\left\lvert z \right\rvert \leq 1$
$f_{c}(z) = z^{2} + c, \quad c \leq 1 \in \mathbb{C}$
$P_{c}$
$Q^{(k)}_{c}$
$k$
$f_{c}$
$\lim_{k \rightarrow \infty} \left[ Q^{(k)}_{c}  \right] = P_{c}$
$E_{c}$
$\infty$
$f_{0}(z) = z^{2}$
$\left\lvert z  \right \rvert \leq 1$
$\left\lvert z  \right \rvert = 1$
$f_{1}(z) = z^{2} - 1$
$f_{0}: z \rightarrow z^{2}$
$f_{c}$
$\left\lvert z \right\rvert >
\mathrm{max}\left(\left\{c, 2\}\right)$
$\left\lvert c \rvert\right \leq 1$
$(k)$
$z$
$f_{0}: z \rightarrow z^{2}$
$f_{1}: z \rightarrow
z^{2} - 1$
$f_{\frac{1}{4} + \frac{i}{2}}: z
\rightarrow z^{2} + (\frac{1}{4} + \frac{i}{2})$
$f_{0}: z \rightarrow z^{2} - 1$
$f_{\frac{1}{4} + \frac{i}{2}}: z \rightarrow z^{2} + \frac{1}{4} + \frac{i}{2}$
$f_{0.8 e^{\pi i \tau}}: z \rightarrow z^{2} + 0.8 e^{\pi
i \tau}, \enspace \tau \in \mathbb{R}$
$\tau$
$f_{0.8 e^{\pi i \tau}}$
$c$
$\left\lvert \gamma \right \rvert < 1$
$f_{\gamma}$
$P$
$z \rightarrow z^{2} + z_{0}$
$z_{0}$
\begin{align}
z_{n+1} &= z^{2}_n + c \label{eq:mb-sequence} \\
z_{0}   &= c
\end{align}
$c$
$\[\[cite:[a-z0-9A-Z]+\]\[.*\]\]$
$cite:[a-z0-9A-Z]+$
$\[\[cite:[a-z0-9A-Z]+\]\[.*\]\]$
$cite:[a-z0-9A-Z]+$
$\[\[cite:[a-z0-9A-Z]+\]\[.*\]\]$
$cite:[a-z0-9A-Z]+$
$\**$
$\* $
\end{document}
%%Local Variables:
%%TeX-master: t
%%End:
