\documentclass{article}
\usepackage[usenames]{color}
\usepackage{minted}
\usepackage[utf8]{inputenc}
\usepackage[T1]{fontenc}
\usepackage{graphicx}
\usepackage{grffile}
% Package longtable omitted
% Package wrapfig omitted
% Package rotating omitted
\usepackage[normalem]{ulem}
\usepackage{amsmath}
\usepackage{textcomp}
\usepackage{amssymb}
% Package capt-of omitted
% Package hyperref omitted
\pagestyle{empty}             % do not remove
% The settings below are copied from fullpage.sty
\setlength{\textwidth}{\paperwidth}
\addtolength{\textwidth}{-3cm}
\setlength{\oddsidemargin}{1.5cm}
\addtolength{\oddsidemargin}{-2.54cm}
\setlength{\evensidemargin}{\oddsidemargin}
\setlength{\textheight}{\paperheight}
\addtolength{\textheight}{-\headheight}
\addtolength{\textheight}{-\headsep}
\addtolength{\textheight}{-\footskip}
\addtolength{\textheight}{-3cm}
\setlength{\topmargin}{1.5cm}
\addtolength{\topmargin}{-2.54cm}

\IfFileExists{./resources/style.sty}{\usepackage{./resources/style}}{}
\IfFileExists{./resources/referencing.sty}{\usepackage{./resources/referencing}}{}
\addbibresource{../Resources/references.bib}
\usepackage[mode=buildnew]{standalone}
\usepackage{tikz}
\usetikzlibrary{decorations.fractals}
\usetikzlibrary{lindenmayersystems}

\begin{document}
$f(x) = xe^x$
\begin{align*}
    xe^x &= 0+\frac{1}{1!}x+\frac{2}{2!}x^2+\frac{3}{3!}x^3+\frac{4}{4!}x^4+\frac{5}{5!}x^5+\dots\\
    &= \sum_{n=0}^\infty \frac{nx^n}{n!}\\
    &= \sum_{n=1}^\infty \frac{x^n}{(n-1)!}
\end{align*}
$f(x) = x^2e^x$
\begin{align*}
    x^2e^x &= \frac{0}{0!} + \frac{0x}{1!} + \frac{2x^2}{2!} + \frac{6x^3}{3!} + \frac{12x^4}{4!} + \frac{20x^5}{5!} + \dots\\
    &= \frac{2\cdot 1x^2}{2!} + \frac{3\cdot 2 x^3}{3!} + \frac{4\cdot 3x^4}{4!} + \frac{5\cdot 4 x^5}{5!} + \dots\\
    &= \sum_{n=2}^\infty \frac{n(n-1)x^n}{n!}\\
    &= \sum_{n=2}^\infty \frac{x^n}{(n-2)!}
\end{align*}
\begin{align*}
    x^ke^x = \sum_{n=k}^\infty \frac{x^n}{(n-k)!} \quad \text{for}~k\in \mathbb{Z^{+}}\cap0
\end{align*}
$f(x) = xe^x$
\begin{align*}
    xe^x &= 0+\frac{1}{1!}x+\frac{2}{2!}x^2+\frac{3}{3!}x^3+\frac{4}{4!}x^4+\frac{5}{5!}x^5+\dots\\
    &= \sum_{n=0}^\infty \frac{nx^n}{n!}\\
    &= \sum_{n=1}^\infty \frac{x^n}{(n-1)!}
\end{align*}
$f(x) = x^2e^x$
\begin{align*}
    x^2e^x &= \frac{0}{0!} + \frac{0x}{1!} + \frac{2x^2}{2!} + \frac{6x^3}{3!} + \frac{12x^4}{4!} + \frac{20x^5}{5!} + \dots\\
    &= \frac{2\cdot 1x^2}{2!} + \frac{3\cdot 2 x^3}{3!} + \frac{4\cdot 3x^4}{4!} + \frac{5\cdot 4 x^5}{5!} + \dots\\
    &= \sum_{n=2}^\infty \frac{n(n-1)x^n}{n!}\\
    &= \sum_{n=2}^\infty \frac{x^n}{(n-2)!}
\end{align*}
\begin{align*}
    x^ke^x = \sum_{n=k}^\infty \frac{x^n}{(n-k)!} \quad \text{for}~k\in \mathbb{Z^{+}}\cap0
\end{align*}
$k=0$
\begin{align*}
    LHS &= x^0e^x = e^x\\
    RHS &= \sum_{n=0}^\infty \frac{x^n}{n!} = e^x\\
\end{align*}
$k=0$
$x^k e^x = \sum_{n=k}^\infty\frac{x^n}{(n-k)!}$
$x^{k+1}e^x = \sum_{n=k+1}^\infty\frac{x^n}{(n-(k+1))!}$
\begin{align*}
    \text{LHS} &= x^{k+1}e^x\\
    &= x\cdot x^{k}e^x\\
    &= x\cdot \sum_{n=k}^\infty\frac{x^n}{(n-k)!} \quad \text{(by assumption)}\\
    &= \sum_{n=k}^\infty\frac{x^{n+1}}{(n-k)!}\\
    &= \sum_{n=k+1}^\infty\frac{x^n}{(n-1-k)!} \quad \text{(re-indexing}~ n\text{)}\\
    &= \sum_{n=k+1}^\infty\frac{x^n}{(n-(k+1))!}\\
    &= RHS
\end{align*}
$f(x) = x^ke^x = \sum_{n=k}^\infty\frac{x^n}{(n-k)!}$
$k \ge 0$
$\Gamma$
$\left(x\right)! = $
\end{document}
%%Local Variables:
%%TeX-master: t
%%End:
