\documentclass{article}
\usepackage[usenames]{color}
\usepackage{minted}
\usepackage[utf8]{inputenc}
\usepackage[T1]{fontenc}
\usepackage{graphicx}
\usepackage{grffile}
% Package longtable omitted
% Package wrapfig omitted
% Package rotating omitted
\usepackage[normalem]{ulem}
\usepackage{amsmath}
\usepackage{textcomp}
\usepackage{amssymb}
% Package capt-of omitted
% Package hyperref omitted
\pagestyle{empty}             % do not remove
% The settings below are copied from fullpage.sty
\setlength{\textwidth}{\paperwidth}
\addtolength{\textwidth}{-3cm}
\setlength{\oddsidemargin}{1.5cm}
\addtolength{\oddsidemargin}{-2.54cm}
\setlength{\evensidemargin}{\oddsidemargin}
\setlength{\textheight}{\paperheight}
\addtolength{\textheight}{-\headheight}
\addtolength{\textheight}{-\headsep}
\addtolength{\textheight}{-\footskip}
\addtolength{\textheight}{-3cm}
\setlength{\topmargin}{1.5cm}
\addtolength{\topmargin}{-2.54cm}

\IfFileExists{./resources/style.sty}{\usepackage{./resources/style}}{}
\IfFileExists{./resources/referencing.sty}{\usepackage{./resources/referencing}}{}
\addbibresource{../Resources/references.bib}
\usepackage[mode=buildnew]{standalone}
\usepackage{tikz}
\usetikzlibrary{decorations.fractals}
\usetikzlibrary{lindenmayersystems}

\begin{document}
\begin{align}
    f\left( x \right) &= \sum^{\infty}_{n= 0}   \left[ a_n \frac{x^n}{n!} \right] \label{eq:exp-pow-series} \\
f'\left( x \right) &= \frac{\mathrm{d} }{\mathrm{d} x}\left( \sum^{\infty}_{n= 0}   \left[ a_n \frac{x^n}{n!} \right]  \right) \nonumber \\
&= \frac{\mathrm{d}}{\mathrm{d} x} \left( a_0 \frac{x^0}{0!} +  a_1 \frac{x^1}{1!} +  a_2 \frac{x^2}{2!}+  a_3 \frac{x^3}{3! } +  \ldots \frac{x^k}{k!} \right) \nonumber \\
&= \sum^{\infty}_{n= 0}   \left[ \frac{\mathrm{d} }{\mathrm{d} x}\left( a_n \frac{x^n}{n!} \right) \right] \nonumber \\
&= \sum^{\infty}_{n= 0}   {\left[{ \frac{a_n}{{\left({ n- 1 }\right)!}} } x^{n- 1}  \right]} \nonumber \\
\implies f'(x) &= \sum^{\infty}_{n= 1}   {\left[{ \frac{x^n}{n!}a_{n+  1} }\right]} \label{eq:exp-pow-series-sol}
\end{align}
\begin{align}
f^{(k)}\left(x\right) = \sum_{n=k}^\infty\frac{a_{n+k}\cdot x^n}{n!} \quad \text{for}~k \ge 0
\end{align}
$f^{(k)}\left(x\right) = \sum_{n=k}^\infty\frac{a_{n+k}\cdot x^n}{n!}$
$k+1$
$f^{(k+1)}(x) = \sum_{n=k+1}^\infty\frac{a_{n+k+1}\cdot x^n}{n!}$
\begin{align*}
    \text{LHS} &= f^{(k+1)}(x)\\
    &= \frac{\mathrm{d}}{\mathrm{d}x}\left(f^{(k)}(x)\right)\\
    &= \frac{\mathrm{d}}{\mathrm{d}x}\left(\sum_{n=k}^\infty\frac{a_{n+k}\cdot x^n}{n!}\right)\quad \text{by assumption}\\
    &= \sum_{n=k}^\infty\frac{a_{n+k}\cdot n\cdot x^{n-1}}{n!}\\
    &= \sum_{n=k}^\infty\frac{a_{n+k}\cdot x^{n-1}}{(n-1)!}\\
    &= \sum_{n=k+1}^\infty\frac{a_{n+k+1}\cdot x^{n}}{n!}\\
    &= \text{RHS}
\end{align*}
$f^{(k)}\left(x\right) = \sum_{n=k}^\infty\frac{a_{n+k}\cdot x^n}{n!} \quad \text{for}~k \ge 0$
\begin{align}
\sum^{n}_{i=0} \left[ c_{i} \cdot f^{(i)}(x) \right] = 0 \label{eq:hom-ode}
\end{align}
$f(x)$
$\frac{\partial }{\partial x}{\left({ f{\left({ x }\right)} }\right)}$
$k$
$k^{\mathrm{th}}$
$k$
$f(x)=c_{i} \cdot e^{m_{i}x}$
$f(x)=c_{i} \cdot x^{j}\cdot e^{m_{i}x}$
$\sum^{k}_{i=0}\left[  c_{i}m^{k-i} \right] = 0$
$\exists i,j \in \mathbb{Z}^{+} \cap \left[0,k\right]$
\begin{align}
\sum^{n}_{i= 0}   \left[ c_i \cdot  a_i \right] = 0, \quad \exists c \in
\mathbb{R}, \enspace \forall i<k\in\mathbb{Z}^+ \nonumber \label{eq:recurrence-relation-def}
\end{align}
\begin{align}
    \sum^{\infty}_{n= 0}   \left[ \sum^{k}_{i= 0}   \left[ \frac{x^n}{n!} c_i a_n \right]  \right]  &= 0 \\
    \sum^{\infty}_{n= 0}    \sum^{k}_{i= 0}    \frac{x^n}{n!} c_i a_n    &= 0 \\
        \sum^{k}_{i= 0} c_i \sum^{\infty}_{n= 0}    \frac{x^n}{n!}  a_n    &= 0
\end{align}
\begin{align}
   \sum^{k}_{i= 0}   \left[ c_i f^{\left( i \right)}\left( x \right) \right]
\end{align}
$f{\left({ x }\right)} \propto e^{m_i x}: \quad m_i \neq m_j \forall i\neq j$
\begin{align}
    f{\left({ x }\right)} = \sum^{k}_{i= 0}   {\left[{ k_i e^{m_i x} }\right]}, \quad \exists m,k \in \mathbb{C} \nonumber
\end{align}
$f{\left({ x }\right)}$
$a_n$
\begin{align}
    \sum^{k}_{i= 0}   {\left[{ k_i e^{m_i x}  }\right]}  &= \sum^{k}_{i= 0}   {\left[{ k_i \sum^{\infty}_{n= 0}   \frac{{\left({ m_i x }\right)}^n}{n!}  }\right]}  \nonumber \\
							 &= \sum^{k}_{i= 0}  \sum^{\infty}_{n= 0}   k_i m_i^n \frac{x^n}{n!} \nonumber\\
							 &=    \sum^{\infty}_{n= 0} \sum^{k}_{i= 0}   k_i m_i^n \frac{x^n}{n!} \nonumber \\
							 &= \sum^{\infty}_{n= 0} {\left[{ \frac{x^n}{n!}  \sum^{k}_{i=0}   {\left[{ k_im^n_i }\right]}  }\right]}, \quad \exists k_i \in \mathbb{C}, \enspace \forall i \in \mathbb{Z}^+\cap {\left[{ 1, k }\right]}     \label{eq:unique-root-sol-power-series-form}
\end{align}
\begin{align}
    f{\left({ x }\right)} &= \sum^{\infty}_{n= 0}   {\left[{  \frac{x^n}{n!} a_n }\right]} \nonumber \\
&= \sum^{\infty}_{n= 0} {\left[{ \frac{x^n}{n!}  \sum^{k}_{i=0}   {\left[{ k_im^n_i }\right]}  }\right]}  \nonumber \\
      \implies  a_n &= \sum^{k}_{n= 0} {\left[{ k_im_i^n }\right]}     \nonumber \\ \nonumber
\square
\end{align}
$m_1 = \varphi, m_2 = {\left({ 1-\varphi }\right)}$
\begin{alignat}{4}
    f{\left({ x }\right)} &= &c_1 e^{\varphi x} +  &c_2 e^{{\left({ 1-\varphi }\right)} x}, \quad &\exists c_1, c_2 \in \mathbb{R} \subset \mathbb{C} \nonumber \\
    \iff  a_n &= &k_1 n^{\varphi} +  &k_2 n^{1- \varphi}, &\exists k_1, k_2 \in \mathbb{R} \subset \mathbb{C} \nonumber
\end{alignat}
\begin{align}
    a_{n+2} -  10a_{n+ 1} +  25a_{n}&= 0 \label{eq:hom-repeated-roots-recurrence} \\
    \implies  \sum^{\infty}_{n= 0}   {\left[{ a_{n+2} \frac{x^n}{n!} }\right]} - 10 \sum^{\infty}_{n= 0}   {\left[{ a_{n+1} \frac{x^n}{n!}    }\right]} + 25 \sum^{\infty}_{n= 0 }   {\left[{  a_{n}\frac{x^n}{n!} }\right]}&= 0 \nonumber
\end{align}
\begin{align}
    f''{\left({ x }\right)}- 10f'{\left({ x }\right)}+  25f{\left({ x }\right)}= 0 \label{eq:rep-roots-func-ode}
\end{align}
\begin{align}
    m^2- 10m+  25 = 0 \nonumber \\
    {\left({ m- 5 }\right)}^2 = 0 \nonumber \\
    m= 5 \label{eq:rep-roots-recurrence-char-sol}
\end{align}
\begin{align}
    f{\left({ x }\right)}= c_1e^{5x} +  c_2 x e^{5x} \label{eq:rep-roots-ode-sol}
\end{align}
\begin{align}
    x^ke^x &= \sum^{\infty}_{n= k}   {\left[{ \frac{x^n}{{\left({ n- k }\right)}!} }\right]}, \quad \exists k \in \mathbb{Z}^+ \label{eq:uniq-roots-pow-series-ident}
\end{align}
\begin{align}
    \implies  f{\left({ x }\right)} &= \sum^{\infty}_{n= 0}   {\left[{ c_1 \frac{{\left({ 5x }\right)}^n}{n!} }\right]}  +  \sum^{\infty}_{n= 1}   {\left[{ c_2 n \frac{{\left({ 5x }\right)^n}}{n{\left({ n-1 }\right)}!} }\right]} \nonumber \\
 &= \sum^{\infty}_{n= 0}   {\left[{ \frac{x^n}{n!} {\left({ c_{1}5^n +  c_2 n 5^n   }\right)} }\right]} \nonumber
\end{align}
\begin{align}
    f{\left({ x }\right)}&=     \sum^{\infty}_{n= 0}   {\left[{ a_n \frac{x^n}{n!} }\right]} \nonumber \\
    \iff a_n &= c_{1}5^n +  c_{2}5^n \nonumber \\ \nonumber
    \ \nonumber \\
    \square \nonumber
\end{align}
\begin{align}
     \sum^{k}_{n= 0}   {\left[{ c_i a_n }\right]}  = 0 \nonumber \\
      \implies  \sum^{\infty}_{n= 0}   \sum^{k}_{i= 0}   c_i a_n \frac{x^n}{n!} = 0 \nonumber \\
      \sum^{k}_{i= 0}   \sum^{\infty}_{n= 0}   c_i a_n \frac{x^n}{n!} \nonumber
\end{align}
\begin{align}
    \sum^{k}_{i= 0}   {\left[{ c_if^{{\left({ k }\right)}}  {\left({ x }\right)}    }\right]} \label{eq:gen-form-rep-roots-ode}
\end{align}
$k$
\begin{align}
			 & \sum^{k}_{i= 0}   {\left[{ c_i m^i }\right]} = 0 \wedge m=B, \enspace  \exists! B \in \mathbb{C} \nonumber \\
 \implies      f{\left({ x }\right)}&= \sum^{k}_{i= 0}   {\left[{ x^i A_i e^{mx} }\right]}, \quad \exists A \in \mathbb{C}^+, \enspace \forall i \in {\left[{ 1,k }\right]} \cap \mathbb{N}  \label{eq:sol-rep-roots-ode}
\end{align}
\begin{align}
x^k e^x = \sum^{\infty}_{n= k} {\left[{ \frac{x^n}{{\left({ n- k }\right)}!} }\right]}  \nonumber
\end{align}
\begin{align}
f{\left({ x }\right)}&=     \sum^{k}_{i= 0}   {\left[{ A_i \sum^{\infty}_{n= i}   {\left[{ \frac{{\left({ x m }\right)}^n}{{\left({ n- i }\right)}!} }\right]}  }\right]} \nonumber \\
&=     \sum^{\infty}_{n= 0}   {\left[{ \sum^{k}_{i=0} {\left[{ \frac{x^n}{n!}  \frac{n!}{{\left({ n- i }\right)!}} A_i m^n }\right]}       }\right]} \nonumber \\
&=     \sum^{\infty}_{n= 0} {\left[{ \frac{x^n}{n!}   \sum^{k}_{i=0} {\left[{  \frac{n!}{{\left({ n- i }\right)!}} A_i m^n }\right]}       }\right]} \nonumber
\end{align}
\begin{align}
f{\left({ x }\right)}&= \sum^{\infty}_{n= 0}   {\left[{ a_n \frac{x^n}{n!} }\right]}      \nonumber \\
 \implies  a_n &= \sum^{k}_{i= 0}   {\left[{ A_i \frac{n!}{{\left({ n- i }\right)}!} m^n  }\right]} \nonumber \\
 &= \sum^{k}_{i= 0}   {\left[{ m^n A_i \prod_{0}^{k} {\left[{ n- {\left({ i- 1 }\right)} }\right]}   }\right]}
& \intertext{$\because \enspace i \leq k$} \notag \nonumber \\
 &= \sum^{k}_{i= 0} {\left[{ A_i^* m^n n^i }\right]}, \quad \exists A_i \in \mathbb{C}, \enspace \forall i\leq k \in \mathbb{Z}^+ \nonumber \\
\ \nonumber \\
\square \nonumber
\end{align}
$f(x) = xe^x$
\begin{align*}
    xe^x &= 0+\frac{1}{1!}x+\frac{2}{2!}x^2+\frac{3}{3!}x^3+\frac{4}{4!}x^4+\frac{5}{5!}x^5+\dots\\
    &= \sum_{n=0}^\infty \frac{nx^n}{n!}\\
    &= \sum_{n=1}^\infty \frac{x^n}{(n-1)!}
\end{align*}
$f(x) = x^2e^x$
\begin{align*}
    x^2e^x &= \frac{0}{0!} + \frac{0x}{1!} + \frac{2x^2}{2!} + \frac{6x^3}{3!} + \frac{12x^4}{4!} + \frac{20x^5}{5!} + \dots\\
    &= \frac{2\cdot 1x^2}{2!} + \frac{3\cdot 2 x^3}{3!} + \frac{4\cdot 3x^4}{4!} + \frac{5\cdot 4 x^5}{5!} + \dots\\
    &= \sum_{n=2}^\infty \frac{n(n-1)x^n}{n!}\\
    &= \sum_{n=2}^\infty \frac{x^n}{(n-2)!}
\end{align*}
\begin{align*}
    x^ke^x = \sum_{n=k}^\infty \frac{x^n}{(n-k)!} \quad \text{for}~k\in \mathbb{Z^{+}}\cap0
\end{align*}
\end{document}
%%Local Variables:
%%TeX-master: t
%%End:
